hol/p4_auxScript.sml
@@ -1864,7 +1864,8 @@ MAP (\(a,b,c,d). c) (ZIP (l,ZIP (l',l''))) = FST (UNZIP l'') /\
 MAP (\(a,b,c,d). d) (ZIP (l,ZIP (l',l''))) = SND (UNZIP l'') /\
 MAP (\(a,b,c,d). (a,b)) (ZIP (l,ZIP (l',l''))) = ZIP (l,l')  /\
 MAP (\(a,b,c,d). (a,c)) (ZIP (l,ZIP (l',l''))) = ZIP (l, FST (UNZIP l'') ) /\
-MAP (\(a,b,c,d). (b,c)) (ZIP (l,ZIP (l',l''))) = ZIP (l', FST (UNZIP l'') )
+MAP (\(a,b,c,d). (b,c)) (ZIP (l,ZIP (l',l''))) = ZIP (l', FST (UNZIP l'') ) /\
+MAP (\(a,b,c,d). (a,b,c)) (ZIP (l,ZIP (l',l''))) = ZIP (l, ZIP ( l' , FST (UNZIP l'') ) )
 )
 Proof
 
